Meta: Class.{Equiv, Incl} test

coq/ZF/Meta/Decl/Class/Equiv.v
@@ -1,109 +1,263 @@
 Require Import Coq.Lists.List.
 Require Import Coq.Strings.String.
 
-Require Import ZF.Meta.Ctx.
-Require Import ZF.Meta.Term.Decl.
 Require Import ZF.Meta.Env.
-Require Import ZF.Meta.Term.CheckDecl.
-Require Import ZF.Meta.Check.
+Require Import ZF.Meta.Proof.Decl.
 Require Import ZF.Meta.Syntax.
+Require Import ZF.Meta.Term.Decl.
 Require Import ZF.Meta.Ty.
 
 Import ListNotations.
 
-(* Declarations.                                                                *)
+(* Term declarations.                                                           *)
 
 (* Definition toClass (a:U) : Class := fun x => x :< a.                         *)
-Definition toClass : Decl :=
-  {| paraT := [TySet];
-     resT  := TyClass;
-     bodyT := Lam (Elem (Var 0) (Var 1)) |}.
+Definition toClass : DeclT :=
+  {| paraT := [TySet]
+  ;  resT  := TyClass
+  ;  bodyT := Lam (Elem (Var 0) (Var 1))
+  |}.
 
 (* Definition equiv (P Q:Class) : Prop := forall x, P x <-> Q x.                *)
-Definition equiv : Decl :=
-  {| paraT := [TyClass; TyClass];
-     resT  := TyProp;
-     bodyT :=
-       (All VarTySet
-         (Iff
-           (App (Var 2) (Var 0))
-           (App (Var 1) (Var 0)))) |}.
+Definition equiv : DeclT :=
+  {| paraT := [TyClass; TyClass]
+  ;  resT  := TyProp
+  ;  bodyT :=
+      All VarTySet
+        (Iff
+          (App (Var 2) (Var 0))
+          (App (Var 1) (Var 0)))
+  |}.
+
+(* Proof declarations                                                           *)
+
+(* Proposition Refl : forall (P:Class), equiv P P.                              *)
+Definition Refl : DeclP :=
+  let concl :=
+      All VarTyClass
+        (IdentT "equiv" [Var 0; Var 0])
+  in
+    {| paraP  := []
+    ;  conclP := concl
+    ;  bodyP  := HoleP concl
+    |}.
+
+(* Proposition EquivCompat : forall A B C D,                                    *)
+(* equiv A C -> equiv B D -> equiv A B -> equiv C D.                            *)
+Definition EquivCompat : DeclP :=
+  let concl :=
+      All VarTyClass
+        (All VarTyClass
+          (All VarTyClass
+            (All VarTyClass
+              (Imp
+                (IdentT "equiv" [Var 3; Var 1])
+                (Imp
+                  (IdentT "equiv" [Var 2; Var 0])
+                  (Imp
+                    (IdentT "equiv" [Var 3; Var 2])
+                    (IdentT "equiv" [Var 1; Var 0])))))))
+  in
+    {| paraP  := []
+    ;  conclP := concl
+    ;  bodyP  := HoleP concl
+    |}.
+
+(* Proposition EquivCompatL : forall A B C,                                     *)
+(* equiv A C -> equiv A B -> equiv C B.                                         *)
+Definition EquivCompatL : DeclP :=
+  let concl :=
+      All VarTyClass
+        (All VarTyClass
+          (All VarTyClass
+            (Imp
+              (IdentT "equiv" [Var 2; Var 0])
+              (Imp
+                (IdentT "equiv" [Var 2; Var 1])
+                (IdentT "equiv" [Var 0; Var 1])))))
+  in
+    {| paraP  := []
+    ;  conclP := concl
+    ;  bodyP  := HoleP concl
+    |}.
+
+(* Proposition EquivCompatR : forall A B C,                                     *)
+(* equiv B C -> equiv A B -> equiv A C.                                         *)
+Definition EquivCompatR : DeclP :=
+  let concl :=
+      All VarTyClass
+        (All VarTyClass
+          (All VarTyClass
+            (Imp
+              (IdentT "equiv" [Var 1; Var 0])
+              (Imp
+                (IdentT "equiv" [Var 2; Var 1])
+                (IdentT "equiv" [Var 2; Var 0])))))
+  in
+    {| paraP  := []
+    ;  conclP := concl
+    ;  bodyP  := HoleP concl
+    |}.
+
+(* Proposition Sym : forall P Q, equiv P Q -> equiv Q P.                        *)
+Definition Sym : DeclP :=
+  let concl :=
+      All VarTyClass
+        (All VarTyClass
+          (Imp
+            (IdentT "equiv" [Var 1; Var 0])
+            (IdentT "equiv" [Var 0; Var 1])))
+  in
+    {| paraP  := []
+    ;  conclP := concl
+    ;  bodyP  := HoleP concl
+    |}.
+
+(* Proposition Tran : forall P Q R,                                             *)
+(* equiv P Q -> equiv Q R -> equiv P R.                                         *)
+Definition Tran : DeclP :=
+  let concl :=
+      All VarTyClass
+        (All VarTyClass
+          (All VarTyClass
+            (Imp
+              (IdentT "equiv" [Var 2; Var 1])
+              (Imp
+                (IdentT "equiv" [Var 1; Var 0])
+                (IdentT "equiv" [Var 2; Var 0])))))
+  in
+    {| paraP  := []
+    ;  conclP := concl
+    ;  bodyP  := HoleP concl
+    |}.
+
+(* Proposition NotSym : forall P Q, ~ equiv P Q -> ~ equiv Q P.                 *)
+Definition NotSym : DeclP :=
+  let concl :=
+      All VarTyClass
+        (All VarTyClass
+          (Imp
+            (Not (IdentT "equiv" [Var 1; Var 0]))
+            (Not (IdentT "equiv" [Var 0; Var 1]))))
+  in
+    {| paraP  := []
+    ;  conclP := concl
+    ;  bodyP  := HoleP concl
+    |}.
+
+(* Proposition EqualToClass : forall a b,                                       *)
+(* a = b <-> equiv (toClass a) (toClass b).                                     *)
+Definition EqualToClass : DeclP :=
+  let concl :=
+      All VarTySet
+        (All VarTySet
+          (Iff
+            (Equal (Var 1) (Var 0))
+            (IdentT "equiv"
+              [IdentT "toClass" [Var 1]; IdentT "toClass" [Var 0]])))
+  in
+    {| paraP  := []
+    ;  conclP := concl
+    ;  bodyP  := HoleP concl
+    |}.
+
+(* Proposition NotEqualToClass : forall a b,                                    *)
+(* a <> b <-> ~ equiv (toClass a) (toClass b).                                  *)
+Definition NotEqualToClass : DeclP :=
+  let concl :=
+      All VarTySet
+        (All VarTySet
+          (Iff
+            (NotEq (Var 1) (Var 0))
+            (Not
+              (IdentT "equiv"
+                [IdentT "toClass" [Var 1]; IdentT "toClass" [Var 0]]))))
+  in
+    {| paraP  := []
+    ;  conclP := concl
+    ;  bodyP  := HoleP concl
+    |}.
+
+(* Proposition NotCompat : forall P Q R S,                                      *)
+(* equiv P Q -> equiv R S -> ~ equiv P R -> ~ equiv Q S.                        *)
+Definition NotCompat : DeclP :=
+  let concl :=
+      All VarTyClass
+        (All VarTyClass
+          (All VarTyClass
+            (All VarTyClass
+              (Imp
+                (IdentT "equiv" [Var 3; Var 2])
+                (Imp
+                  (IdentT "equiv" [Var 1; Var 0])
+                  (Imp
+                    (Not (IdentT "equiv" [Var 3; Var 1]))
+                    (Not (IdentT "equiv" [Var 2; Var 0]))))))))
+  in
+    {| paraP  := []
+    ;  conclP := concl
+    ;  bodyP  := HoleP concl
+    |}.
+
+(* Proposition NotCompatL : forall P Q R,                                       *)
+(* equiv P Q -> ~ equiv P R -> ~ equiv Q R.                                     *)
+Definition NotCompatL : DeclP :=
+  let concl :=
+      All VarTyClass
+        (All VarTyClass
+          (All VarTyClass
+            (Imp
+              (IdentT "equiv" [Var 2; Var 1])
+              (Imp
+                (Not (IdentT "equiv" [Var 2; Var 0]))
+                (Not (IdentT "equiv" [Var 1; Var 0]))))))
+  in
+    {| paraP  := []
+    ;  conclP := concl
+    ;  bodyP  := HoleP concl
+    |}.
+
+(* Proposition NotCompatR : forall P Q R,                                       *)
+(* equiv P Q -> ~ equiv R P -> ~ equiv R Q.                                     *)
+Definition NotCompatR : DeclP :=
+  let concl :=
+      All VarTyClass
+        (All VarTyClass
+          (All VarTyClass
+            (Imp
+              (IdentT "equiv" [Var 2; Var 1])
+              (Imp
+                (Not (IdentT "equiv" [Var 0; Var 2]))
+                (Not (IdentT "equiv" [Var 0; Var 1]))))))
+  in
+    {| paraP  := []
+    ;  conclP := concl
+    ;  bodyP  := HoleP concl
+    |}.
 
 (* Environment.                                                                 *)
 
 Definition imports : Env := Env.empty.
 
-Definition exports : Env := Env.fromListT
-  [ ("toClass"%string, toClass)
-  ; ("equiv"%string  , equiv)
+Definition exports : Env := Env.unions
+  [ Env.fromListT
+    [ ("toClass"%string, toClass)
+    ; ("equiv"%string  , equiv)
+    ]
+  ; Env.fromListP
+    [ ("Refl"%string           , Refl)
+    ; ("EquivCompat"%string    , EquivCompat)
+    ; ("EquivCompatL"%string   , EquivCompatL)
+    ; ("EquivCompatR"%string   , EquivCompatR)
+    ; ("Sym"%string            , Sym)
+    ; ("Tran"%string           , Tran)
+    ; ("NotSym"%string         , NotSym)
+    ; ("EqualToClass"%string   , EqualToClass)
+    ; ("NotEqualToClass"%string, NotEqualToClass)
+    ; ("NotCompat"%string      , NotCompat)
+    ; ("NotCompatL"%string     , NotCompatL)
+    ; ("NotCompatR"%string     , NotCompatR)
+    ]
   ].
 
 Definition env : Env := Env.union imports exports.
-
-(* Body checks.                                                                 *)
-
-(* The declaration body for toClass maps a set to its membership class.         *)
-Proposition toClassCheckBody : CheckDecl Env.empty toClass.
-Proof.
-  (* Proof by Hermes + gpt 5.5                                                  *)
-  apply CheckLam, CheckElem; apply CheckVar; reflexivity.
-Qed.
-
-(* The declaration body for equivalence compares two classes pointwise.         *)
-Proposition equivCheckBody : CheckDecl Env.empty equiv.
-Proof.
-  (* Proof by Hermes + gpt 5.5                                                  *)
-  apply CheckAll, CheckIff.
-  - apply CheckApp.
-    + apply CheckVar. reflexivity.
-    + apply CheckVar. reflexivity.
-  - apply CheckApp.
-    + apply CheckVar. reflexivity.
-    + apply CheckVar. reflexivity.
-Qed.
-
-(* Identifier checks.                                                           *)
-
-(* The identifier toClass sends any set variable to a class in any environment. *)
-Proposition toClassCheckIdent : forall (e:Env) (G:Ctx) (n:nat),
-  Env.sigT e "toClass"%string = Some ([TySet], TyClass) ->
-  typeOf G n = Some TySet ->
-  CheckT e G (IdentT "toClass" [Var n]) TyClass.
-Proof.
-  (* Proof by Hermes + gpt 5.5                                                  *)
-  intros e G n H1 H2.
-  apply CheckIdentT with [TySet]. 1: assumption.
-  - apply CheckTsCons.
-    + apply CheckVar. assumption.
-    + apply CheckTsNil.
-Qed.
-
-(* Equivalence applied to two class variables is well sorted anywhere.          *)
-Proposition equivCheckIdent : forall (e:Env) (G:Ctx) (m n:nat),
-  Env.sigT e "equiv"%string = Some ([TyClass; TyClass], TyProp) ->
-  typeOf G m = Some TyClass ->
-  typeOf G n = Some TyClass ->
-  CheckT e G (IdentT "equiv" [Var m; Var n]) TyProp.
-Proof.
-  (* Proof by Hermes + gpt 5.5                                                  *)
-  intros e G m n H1 H2 H3.
-  apply CheckIdentT with [TyClass;TyClass]. 1: assumption.
-  - apply CheckTsCons.
-    + apply CheckVar. assumption.
-    + apply CheckTsCons.
-      * apply CheckVar. assumption.
-      * apply CheckTsNil.
-Qed.
-
-(* Negated equivalence of two class variables is well sorted anywhere.          *)
-Proposition notEquivCheckIdent : forall (e:Env) (G:Ctx) (m n:nat),
-  Env.sigT e "equiv"%string = Some ([TyClass; TyClass], TyProp) ->
-  typeOf G m = Some TyClass ->
-  typeOf G n = Some TyClass ->
-  CheckT e G (Not (IdentT "equiv" [Var m; Var n])) TyProp.
-Proof.
-  (* Proof by Hermes + gpt 5.5                                                  *)
-  intros e G m n H1 H2 H3.
-  apply CheckNot.
-  apply equivCheckIdent; assumption.
-Qed.
